v0.12.0

bin/lunno.ml
@@ -1,1 +1,14 @@
-let () = Printf.printf "Lunno\n"
+open Lunno_driver
+open Lunno_debug
+
+let () =
+  let args = Array.to_list Sys.argv |> List.tl in
+  if args = [] then begin
+    Printf.eprintf "Usage: lunno <file.ln> [...]\n";
+    exit 1
+  end;
+  List.iter
+    (fun path ->
+      let prog = Cli.parse_file path in
+      Debug.dump_program prog)
+    args
