lib/common/span.ml
@@ -1,0 +1,11 @@
+type pos = { line : int; col : int }
+type span = { start : pos; stop : pos }
+
+let dummy_pos = { line = 0; col = 0 }
+let dummy_span = { start = dummy_pos; stop = dummy_pos }
+let string_of_pos p = Printf.sprintf "%d:%d" p.line p.col
+
+let string_of_span s =
+  Printf.sprintf "[%s-%s]" (string_of_pos s.start) (string_of_pos s.stop)
+
+let merge a b = { start = a.start; stop = b.stop }
