lib/common/span.mli
@@ -1,0 +1,8 @@
+type pos = { line : int; col : int }
+type span = { start : pos; stop : pos }
+
+val dummy_pos : pos
+val dummy_span : span
+val string_of_pos : pos -> string
+val string_of_span : span -> string
+val merge : span -> span -> span
