lib/common/util.mli
@@ -1,0 +1,2 @@
+val coq_string_to_string : char list -> string
+val ocaml_string_to_coq : string -> char list
