lib/debug/debug.mli
@@ -1,0 +1,1 @@
+val dump_program : Lunno_frontend.Spanned_ast.program -> unit
