lib/frontend/positioned_lexer.ml
@@ -1,0 +1,124 @@
+open Lunno_common
+
+let build_pos_table src =
+  let n = String.length src in
+  let tbl = Array.make n Span.dummy_pos in
+  let line = ref 1 in
+  let col = ref 1 in
+  for i = 0 to n - 1 do
+    tbl.(i) <- { Span.line = !line; col = !col };
+    if src.[i] = '\n' then begin
+      incr line;
+      col := 1
+    end
+    else incr col
+  done;
+  tbl
+
+let token_extent src tok offset =
+  let n = String.length src in
+  let rec skip_ws i =
+    if i >= n then i
+    else
+      match src.[i] with
+      | ' ' | '\t' | '\r' | '\n' -> skip_ws (i + 1)
+      | '#' ->
+          let rec skip_line j =
+            if j >= n || src.[j] = '\n' then skip_ws (j + 1)
+            else skip_line (j + 1)
+          in
+          skip_line (i + 1)
+      | _ -> i
+  in
+  let start = skip_ws offset in
+  let stop =
+    match tok with
+    | Lunno.TEOF -> start
+    | Lunno.TIntLit _ ->
+        let j = ref start in
+        while !j < n && src.[!j] >= '0' && src.[!j] <= '9' do
+          incr j
+        done;
+        if
+          !j + 1 < n
+          && src.[!j] = '.'
+          && src.[!j + 1] >= '0'
+          && src.[!j + 1] <= '9'
+        then begin
+          incr j;
+          while !j < n && src.[!j] >= '0' && src.[!j] <= '9' do
+            incr j
+          done
+        end;
+        !j
+    | Lunno.TFloatLit _ ->
+        let j = ref start in
+        while !j < n && src.[!j] >= '0' && src.[!j] <= '9' do
+          incr j
+        done;
+        if !j < n && src.[!j] = '.' then begin
+          incr j;
+          while !j < n && src.[!j] >= '0' && src.[!j] <= '9' do
+            incr j
+          done
+        end;
+        !j
+    | Lunno.TStringLit _ ->
+        let j = ref (start + 1) in
+        while !j < n && src.[!j] <> '"' do
+          if src.[!j] = '\\' then incr j;
+          incr j
+        done;
+        !j + 1
+    | Lunno.TIdent s ->
+        let _ = s in
+        let j = ref start in
+        let is_ident_char c =
+          (c >= 'a' && c <= 'z')
+          || (c >= 'A' && c <= 'Z')
+          || (c >= '0' && c <= '9')
+          || c = '_'
+        in
+        while !j < n && is_ident_char src.[!j] do
+          incr j
+        done;
+        !j
+    | Lunno.TArrow | Lunno.TNotEq | Lunno.TCons | Lunno.TDotDot -> start + 2
+    | _ ->
+        let j = ref start in
+        let is_ident_char c =
+          (c >= 'a' && c <= 'z')
+          || (c >= 'A' && c <= 'Z')
+          || (c >= '0' && c <= '9')
+          || c = '_'
+        in
+        if start < n && is_ident_char src.[start] then begin
+          while !j < n && is_ident_char src.[!j] do
+            incr j
+          done
+        end
+        else incr j;
+        !j
+  in
+  (start, stop)
+
+let position_tokens src tokens =
+  let tbl = build_pos_table src in
+  let n = String.length src in
+  let pos_of i =
+    if i < n then tbl.(i)
+    else { Span.line = tbl.(n - 1).Span.line; col = tbl.(n - 1).Span.col + 1 }
+  in
+  let offset = ref 0 in
+  List.map
+    (fun tok ->
+      let lo, hi = token_extent src tok !offset in
+      let sp = { Span.start = pos_of lo; stop = pos_of hi } in
+      offset := hi;
+      (tok, sp))
+    tokens
+
+let lex src =
+  match Lunno.lex (Util.ocaml_string_to_coq src) with
+  | Lunno.LexErr msg -> Error (Util.coq_string_to_string msg)
+  | Lunno.LexOk tokens -> Ok (position_tokens src tokens)
