lib/frontend/positioned_lexer.mli
@@ -1,0 +1,6 @@
+open Lunno_common
+
+val position_tokens :
+  string -> Lunno.token list -> (Lunno.token * Span.span) list
+
+val lex : string -> ((Lunno.token * Span.span) list, string) result
