lib/frontend/span_parser.ml
@@ -1,0 +1,228 @@
+open Lunno_common
+
+type cursor = { mutable toks : (Lunno.token * Span.span) list }
+
+let make_cursor toks = { toks }
+let peek cur = match cur.toks with [] -> None | (t, _) :: _ -> Some t
+
+let peek_span cur =
+  match cur.toks with [] -> Span.dummy_span | (_, sp) :: _ -> sp
+
+let advance cur = match cur.toks with [] -> () | _ :: tl -> cur.toks <- tl
+
+let consume cur =
+  match cur.toks with
+  | [] -> Span.dummy_span
+  | (_, sp) :: tl ->
+      cur.toks <- tl;
+      sp
+
+let consume_if cur tok =
+  match cur.toks with
+  | (t, _) :: tl when Lunno.token_beq t tok -> cur.toks <- tl
+  | _ -> ()
+
+let coq = Util.coq_string_to_string
+
+let rec attach_expr cur e =
+  match e with
+  | Lunno.Lit l ->
+      let sp = consume cur in
+      Spanned_ast.Lit (l, sp)
+  | Lunno.Var nm ->
+      let sp = consume cur in
+      Spanned_ast.Var (coq nm, sp)
+  | Lunno.LetE (nm, ty, body) ->
+      let sp_start = consume cur in
+      advance cur;
+      (match peek cur with
+      | Some Lunno.TColon ->
+          consume_if cur Lunno.TColon;
+          skip_ty cur ty;
+          consume_if cur Lunno.TEquals
+      | Some Lunno.TEquals -> consume_if cur Lunno.TEquals
+      | Some Lunno.TLParen -> (
+          consume_if cur Lunno.TLParen;
+          skip_params cur body;
+          consume_if cur Lunno.TRParen;
+          match peek cur with
+          | Some Lunno.TArrow ->
+              consume_if cur Lunno.TArrow;
+              skip_ty cur ty
+          | _ -> ())
+      | Some Lunno.TLBrace -> ()
+      | _ -> ());
+      let body' = attach_expr cur body in
+      let sp = Span.merge sp_start (Spanned_ast.span_of body') in
+      Spanned_ast.LetE (coq nm, ty, body', sp)
+  | Lunno.Lam (params, ret_ty, body, is_rec) ->
+      let sp_start = peek_span cur in
+      let body' = attach_expr cur body in
+      let sp = Span.merge sp_start (Spanned_ast.span_of body') in
+      Spanned_ast.Lam (params, ret_ty, body', is_rec, sp)
+  | Lunno.App (f, args) ->
+      let f' = attach_expr cur f in
+      consume_if cur Lunno.TLParen;
+      let args' = attach_expr_list cur args in
+      let sp_end = consume cur in
+      let sp = Span.merge (Spanned_ast.span_of f') sp_end in
+      Spanned_ast.App (f', args', sp)
+  | Lunno.IfE (cond, then_, else_) ->
+      let sp_start = consume cur in
+      let cond' = attach_expr cur cond in
+      consume_if cur Lunno.TThen;
+      let then_' = attach_expr cur then_ in
+      let else_', sp_end =
+        match else_ with
+        | None -> (None, Spanned_ast.span_of then_')
+        | Some e ->
+            consume_if cur Lunno.TElse;
+            let e' = attach_expr cur e in
+            (Some e', Spanned_ast.span_of e')
+      in
+      Spanned_ast.IfE (cond', then_', else_', Span.merge sp_start sp_end)
+  | Lunno.MatchE (scrut, cases) ->
+      let sp_start = consume cur in
+      let scrut' = attach_expr cur scrut in
+      consume_if cur Lunno.TLBrace;
+      let cases' = List.map (attach_case cur) cases in
+      let sp_end = consume cur in
+      Spanned_ast.MatchE (scrut', cases', Span.merge sp_start sp_end)
+  | Lunno.Block exprs ->
+      let sp_start = consume cur in
+      let exprs' = List.map (attach_expr cur) exprs in
+      let sp_end = consume cur in
+      let sp =
+        match exprs' with
+        | [] -> Span.merge sp_start sp_end
+        | _ -> Span.merge sp_start sp_end
+      in
+      Spanned_ast.Block (exprs', sp)
+  | Lunno.BinOp (op, l, r) ->
+      let l' = attach_expr cur l in
+      advance cur;
+      let r' = attach_expr cur r in
+      let sp = Span.merge (Spanned_ast.span_of l') (Spanned_ast.span_of r') in
+      Spanned_ast.BinOp (op, l', r', sp)
+  | Lunno.UnOp (op, e) ->
+      let sp_start = consume cur in
+      let e' = attach_expr cur e in
+      Spanned_ast.UnOp (op, e', Span.merge sp_start (Spanned_ast.span_of e'))
+  | Lunno.MemberAccess (obj, field) ->
+      let obj' = attach_expr cur obj in
+      consume_if cur Lunno.TDot;
+      let sp_end = consume cur in
+      Spanned_ast.MemberAccess
+        (obj', coq field, Span.merge (Spanned_ast.span_of obj') sp_end)
+  | Lunno.Range (lo, hi) ->
+      consume_if cur Lunno.TLBracket;
+      let lo' = attach_expr cur lo in
+      consume_if cur Lunno.TDotDot;
+      let hi' = attach_expr cur hi in
+      let sp_end = consume cur in
+      Spanned_ast.Range (lo', hi', Span.merge (Spanned_ast.span_of lo') sp_end)
+  | Lunno.Constructor (nm, args) ->
+      let sp_start = consume cur in
+      consume_if cur Lunno.TLParen;
+      let args' = attach_expr_list cur args in
+      let sp_end = consume cur in
+      Spanned_ast.Constructor (coq nm, args', Span.merge sp_start sp_end)
+
+and attach_expr_list cur = function
+  | [] -> []
+  | [ e ] -> [ attach_expr cur e ]
+  | e :: rest ->
+      let e' = attach_expr cur e in
+      consume_if cur Lunno.TComma;
+      e' :: attach_expr_list cur rest
+
+and attach_case cur (Lunno.MkCase (pat, guard, case_body)) =
+  let sp_start = consume cur in
+  advance cur;
+  let guard' =
+    match guard with
+    | None -> None
+    | Some g ->
+        consume_if cur Lunno.TIf;
+        Some (attach_expr cur g)
+  in
+  consume_if cur Lunno.TArrow;
+  let body' = attach_expr cur case_body in
+  let sp = Span.merge sp_start (Spanned_ast.span_of body') in
+  { Spanned_ast.pat; guard = guard'; case_body = body'; case_span = sp }
+
+and skip_ty cur _ty =
+  let rec go () =
+    match peek cur with
+    | Some Lunno.TInt
+    | Some Lunno.TFloat
+    | Some Lunno.TString
+    | Some Lunno.TBool
+    | Some Lunno.TUnit
+    | Some Lunno.TList
+    | Some (Lunno.TIdent _) ->
+        advance cur;
+        go ()
+    | Some Lunno.TLParen ->
+        advance cur;
+        go ();
+        consume_if cur Lunno.TRParen
+    | _ -> ()
+  in
+  go ()
+
+and skip_params cur _body =
+  let rec go () =
+    match peek cur with
+    | Some (Lunno.TIdent _) -> (
+        advance cur;
+        (match peek cur with
+        | Some Lunno.TColon ->
+            advance cur;
+            skip_ty cur None
+        | _ -> ());
+        match peek cur with
+        | Some Lunno.TComma ->
+            advance cur;
+            go ()
+        | _ -> ())
+    | _ -> ()
+  in
+  go ()
+
+let attach_import cur imp =
+  let sp_start = consume cur in
+  let sp_end = consume cur in
+  let path = coq imp.Lunno.import_module in
+  let module_, item =
+    match String.split_on_char ':' path with
+    | [ m; i ] -> (m, i)
+    | _ -> (path, "")
+  in
+  {
+    Spanned_ast.import_module = module_;
+    import_item = item;
+    import_span = Span.merge sp_start sp_end;
+  }
+
+let attach_program prog positioned =
+  let cur = make_cursor positioned in
+  let imports = List.map (attach_import cur) prog.Lunno.imports in
+  let type_decls =
+    List.map
+      (fun td ->
+        {
+          Spanned_ast.type_name = coq td.Lunno.type_name;
+          variants =
+            List.map
+              (fun v ->
+                {
+                  Spanned_ast.variant_name = coq v.Lunno.variant_name;
+                  variant_fields = v.Lunno.variant_fields;
+                })
+              td.Lunno.variants;
+        })
+      prog.Lunno.type_decls
+  in
+  let body = List.map (attach_expr cur) prog.Lunno.body in
+  { Spanned_ast.imports; type_decls; body }
