lib/frontend/span_parser.mli
@@ -1,0 +1,4 @@
+val attach_program :
+  Lunno.program ->
+  (Lunno.token * Lunno_common.Span.span) list ->
+  Spanned_ast.program
