lib/frontend/spanned_ast.mli
@@ -1,0 +1,44 @@
+open Lunno_common
+
+type ty = Lunno.ty
+type pattern = Lunno.pattern
+type param = Lunno.param
+
+type import = {
+  import_module : string;
+  import_item : string;
+  import_span : Span.span;
+}
+
+type variant = { variant_name : string; variant_fields : ty list }
+type type_decl = { type_name : string; variants : variant list }
+
+type expr =
+  | Lit of Lunno.literal * Span.span
+  | Var of string * Span.span
+  | Lam of param list * ty option * expr * bool * Span.span
+  | App of expr * expr list * Span.span
+  | LetE of string * ty option * expr * Span.span
+  | IfE of expr * expr * expr option * Span.span
+  | MatchE of expr * match_case list * Span.span
+  | Block of expr list * Span.span
+  | BinOp of Lunno.binary_op * expr * expr * Span.span
+  | UnOp of Lunno.unary_op * expr * Span.span
+  | MemberAccess of expr * string * Span.span
+  | Range of expr * expr * Span.span
+  | Constructor of string * expr list * Span.span
+
+and match_case = {
+  pat : pattern;
+  guard : expr option;
+  case_body : expr;
+  case_span : Span.span;
+}
+
+type program = {
+  imports : import list;
+  type_decls : type_decl list;
+  body : expr list;
+}
+
+val span_of : expr -> Span.span
