coq/Lexer.v
@@ -3,6 +3,7 @@ From Stdlib Require Import Strings.Ascii.
 From Stdlib Require Import ZArith.ZArith.
 From Stdlib Require Import Lists.List.
 From Stdlib Require Import Bool.Bool.
+From Stdlib Require Import Lia.
 Import ListNotations.
 
 Require Import Token.
@@ -34,20 +35,21 @@ Definition digit_val (c : ascii) : Z :=
   Z.of_nat (ascii_to_nat c) - 48.
 
 Definition keyword_or_ident (s : string) : token :=
-  if String.eqb s "let"    then TLet
-  else if String.eqb s "if"     then TIf
-  else if String.eqb s "then"   then TThen
-  else if String.eqb s "else"   then TElse
-  else if String.eqb s "match"  then TMatch
+  if String.eqb s "let" then TLet
+  else if String.eqb s "if" then TIf
+  else if String.eqb s "then" then TThen
+  else if String.eqb s "else" then TElse
+  else if String.eqb s "match" then TMatch
   else if String.eqb s "import" then TImport
-  else if String.eqb s "true"   then TTrue
-  else if String.eqb s "false"  then TFalse
-  else if String.eqb s "int"    then TInt
-  else if String.eqb s "float"  then TFloat
+  else if String.eqb s "data" then TData
+  else if String.eqb s "true" then TTrue
+  else if String.eqb s "false" then TFalse
+  else if String.eqb s "int" then TInt
+  else if String.eqb s "float" then TFloat
   else if String.eqb s "string" then TString
-  else if String.eqb s "bool"   then TBool
-  else if String.eqb s "unit"   then TUnit
-  else if String.eqb s "list"   then TList
+  else if String.eqb s "bool" then TBool
+  else if String.eqb s "unit" then TUnit
+  else if String.eqb s "list" then TList
   else TIdent s.
 
 Definition input := list ascii.
@@ -58,7 +60,7 @@ Inductive lex_result : Type :=
 
 Fixpoint take_while (p : ascii -> bool) (cs : input) : (list ascii * input) :=
   match cs with
-  | []      => ([], [])
+  | [] => ([], [])
   | c :: rest =>
       if p c then
         let (taken, remaining) := take_while p rest in
@@ -72,19 +74,19 @@ Definition list_ascii_to_string (cs : list ascii) : string :=
 
 Fixpoint parse_int (cs : list ascii) (acc : Z) : Z :=
   match cs with
-  | []      => acc
+  | [] => acc
   | c :: rest => parse_int rest (acc * 10 + digit_val c)
   end.
 
 Fixpoint lex_string_lit (cs : input) (acc : list ascii) : option (string * input) :=
   match cs with
-  | []              => None
+  | [] => None
   | c :: rest =>
       if Ascii.eqb c """"%char then
         Some (list_ascii_to_string (rev acc), rest)
       else if Ascii.eqb c "\"%char then
         match rest with
-        | []        => None
+        | [] => None
         | e :: rest' =>
             let escaped :=
               if Ascii.eqb e "n"%char  then "010"%char
@@ -101,8 +103,8 @@ Fixpoint lex_string_lit (cs : input) (acc : list ascii) : option (string * input
 
 Fixpoint lex_aux (fuel : nat) (cs : input) (acc : list token) : lex_result :=
   match fuel with
-  | O    => LexErr "lexer out of fuel"
-  | S f  =>
+  | O => LexErr "lexer out of fuel"
+  | S f =>
     match cs with
     | [] => LexOk (rev (TEOF :: acc))
     | c :: rest =>
@@ -112,7 +114,7 @@ Fixpoint lex_aux (fuel : nat) (cs : input) (acc : list token) : lex_result :=
         lex_aux f rest' acc
       else if Ascii.eqb c """"%char then
         match lex_string_lit rest [] with
-        | None           => LexErr "unterminated string literal"
+        | None => LexErr "unterminated string literal"
         | Some (s, rest') => lex_aux f rest' (TStringLit s :: acc)
         end
       else if is_digit c then
@@ -157,44 +159,44 @@ Fixpoint lex_aux (fuel : nat) (cs : input) (acc : list token) : lex_result :=
       else if Ascii.eqb c "-"%char then
         match rest with
         | next :: rest' =>
-          if Ascii.eqb next ">"%char then lex_aux f rest' (TArrow   :: acc)
-          else                             lex_aux f rest  (TMinus   :: acc)
+          if Ascii.eqb next ">"%char then lex_aux f rest' (TArrow :: acc)
+          else lex_aux f rest  (TMinus :: acc)
         | [] => lex_aux f rest (TMinus :: acc)
         end
       else if Ascii.eqb c "<"%char then
         match rest with
         | next :: rest' =>
           if Ascii.eqb next ">"%char then lex_aux f rest' (TNotEq :: acc)
-          else                             lex_aux f rest  (TLt    :: acc)
+          else lex_aux f rest  (TLt :: acc)
         | [] => lex_aux f rest (TLt :: acc)
         end
       else if Ascii.eqb c ">"%char then lex_aux f rest (TGt :: acc)
       else if Ascii.eqb c ":"%char then
         match rest with
         | next :: rest' =>
-          if Ascii.eqb next ":"%char then lex_aux f rest' (TCons   :: acc)
-          else                             lex_aux f rest  (TColon  :: acc)
+          if Ascii.eqb next ":"%char then lex_aux f rest' (TCons :: acc)
+          else lex_aux f rest  (TColon :: acc)
         | [] => lex_aux f rest (TColon :: acc)
         end
       else if Ascii.eqb c "."%char then
         match rest with
         | next :: rest' =>
           if Ascii.eqb next "."%char then lex_aux f rest' (TDotDot :: acc)
-          else                             lex_aux f rest  (TDot    :: acc)
+          else lex_aux f rest  (TDot :: acc)
         | [] => lex_aux f rest (TDot :: acc)
         end
-      else if Ascii.eqb c "("%char  then lex_aux f rest (TLParen   :: acc)
-      else if Ascii.eqb c ")"%char  then lex_aux f rest (TRParen   :: acc)
-      else if Ascii.eqb c "["%char  then lex_aux f rest (TLBracket :: acc)
-      else if Ascii.eqb c "]"%char  then lex_aux f rest (TRBracket :: acc)
-      else if Ascii.eqb c "{"%char  then lex_aux f rest (TLBrace   :: acc)
-      else if Ascii.eqb c "}"%char  then lex_aux f rest (TRBrace   :: acc)
-      else if Ascii.eqb c "+"%char  then lex_aux f rest (TPlus     :: acc)
-      else if Ascii.eqb c "*"%char  then lex_aux f rest (TStar     :: acc)
-      else if Ascii.eqb c "/"%char  then lex_aux f rest (TSlash    :: acc)
-      else if Ascii.eqb c "="%char  then lex_aux f rest (TEquals   :: acc)
-      else if Ascii.eqb c ","%char  then lex_aux f rest (TComma    :: acc)
-      else if Ascii.eqb c "|"%char  then lex_aux f rest (TPipe     :: acc)
+      else if Ascii.eqb c "("%char then lex_aux f rest (TLParen :: acc)
+      else if Ascii.eqb c ")"%char then lex_aux f rest (TRParen :: acc)
+      else if Ascii.eqb c "["%char then lex_aux f rest (TLBracket :: acc)
+      else if Ascii.eqb c "]"%char then lex_aux f rest (TRBracket :: acc)
+      else if Ascii.eqb c "{"%char then lex_aux f rest (TLBrace :: acc)
+      else if Ascii.eqb c "}"%char then lex_aux f rest (TRBrace :: acc)
+      else if Ascii.eqb c "+"%char then lex_aux f rest (TPlus :: acc)
+      else if Ascii.eqb c "*"%char then lex_aux f rest (TStar :: acc)
+      else if Ascii.eqb c "/"%char then lex_aux f rest (TSlash :: acc)
+      else if Ascii.eqb c "="%char then lex_aux f rest (TEquals :: acc)
+      else if Ascii.eqb c ","%char then lex_aux f rest (TComma :: acc)
+      else if Ascii.eqb c "|"%char then lex_aux f rest (TPipe :: acc)
       else LexErr ("unexpected character: " ++ String c EmptyString)
     end
   end.
@@ -204,94 +206,3 @@ Definition string_to_input (s : string) : input :=
 
 Definition lex (src : string) : lex_result :=
   lex_aux (String.length src + 1) (string_to_input src) [].
-
-Lemma lex_empty : lex "" = LexOk [TEOF].
-Proof. reflexivity. Qed.
-
-Lemma lex_let : lex "let" = LexOk [TLet; TEOF].
-Proof. reflexivity. Qed.
-
-Lemma lex_if     : lex "if"     = LexOk [TIf;     TEOF]. Proof. reflexivity. Qed.
-Lemma lex_then   : lex "then"   = LexOk [TThen;   TEOF]. Proof. reflexivity. Qed.
-Lemma lex_else   : lex "else"   = LexOk [TElse;   TEOF]. Proof. reflexivity. Qed.
-Lemma lex_match  : lex "match"  = LexOk [TMatch;  TEOF]. Proof. reflexivity. Qed.
-Lemma lex_import : lex "import" = LexOk [TImport; TEOF]. Proof. reflexivity. Qed.
-Lemma lex_true   : lex "true"   = LexOk [TTrue;   TEOF]. Proof. reflexivity. Qed.
-Lemma lex_false  : lex "false"  = LexOk [TFalse;  TEOF]. Proof. reflexivity. Qed.
-
-Lemma lex_int_kw    : lex "int"    = LexOk [TInt;    TEOF]. Proof. reflexivity. Qed.
-Lemma lex_float_kw  : lex "float"  = LexOk [TFloat;  TEOF]. Proof. reflexivity. Qed.
-Lemma lex_string_kw : lex "string" = LexOk [TString; TEOF]. Proof. reflexivity. Qed.
-Lemma lex_bool_kw   : lex "bool"   = LexOk [TBool;   TEOF]. Proof. reflexivity. Qed.
-Lemma lex_unit_kw   : lex "unit"   = LexOk [TUnit;   TEOF]. Proof. reflexivity. Qed.
-Lemma lex_list_kw   : lex "list"   = LexOk [TList;   TEOF]. Proof. reflexivity. Qed.
-
-Lemma lex_arrow  : lex "->" = LexOk [TArrow;  TEOF]. Proof. reflexivity. Qed.
-Lemma lex_lt     : lex "<"  = LexOk [TLt;    TEOF]. Proof. reflexivity. Qed.
-Lemma lex_gt     : lex ">"  = LexOk [TGt;    TEOF]. Proof. reflexivity. Qed.
-Lemma lex_noteq  : lex "<>" = LexOk [TNotEq; TEOF]. Proof. reflexivity. Qed.
-Lemma lex_cons   : lex "::" = LexOk [TCons;   TEOF]. Proof. reflexivity. Qed.
-Lemma lex_dotdot : lex ".." = LexOk [TDotDot; TEOF]. Proof. reflexivity. Qed.
-
-Lemma lex_plus    : lex "+" = LexOk [TPlus;    TEOF]. Proof. reflexivity. Qed.
-Lemma lex_minus   : lex "-" = LexOk [TMinus;   TEOF]. Proof. reflexivity. Qed.
-Lemma lex_star    : lex "*" = LexOk [TStar;    TEOF]. Proof. reflexivity. Qed.
-Lemma lex_slash   : lex "/" = LexOk [TSlash;   TEOF]. Proof. reflexivity. Qed.
-Lemma lex_equals  : lex "=" = LexOk [TEquals;  TEOF]. Proof. reflexivity. Qed.
-Lemma lex_pipe    : lex "|" = LexOk [TPipe;    TEOF]. Proof. reflexivity. Qed.
-Lemma lex_colon   : lex ":" = LexOk [TColon;   TEOF]. Proof. reflexivity. Qed.
-Lemma lex_dot     : lex "." = LexOk [TDot;     TEOF]. Proof. reflexivity. Qed.
-Lemma lex_comma   : lex "," = LexOk [TComma;   TEOF]. Proof. reflexivity. Qed.
-Lemma lex_lparen  : lex "(" = LexOk [TLParen;  TEOF]. Proof. reflexivity. Qed.
-Lemma lex_rparen  : lex ")" = LexOk [TRParen;  TEOF]. Proof. reflexivity. Qed.
-Lemma lex_lbrack  : lex "[" = LexOk [TLBracket;TEOF]. Proof. reflexivity. Qed.
-Lemma lex_rbrack  : lex "]" = LexOk [TRBracket;TEOF]. Proof. reflexivity. Qed.
-Lemma lex_lbrace  : lex "{" = LexOk [TLBrace;  TEOF]. Proof. reflexivity. Qed.
-Lemma lex_rbrace  : lex "}" = LexOk [TRBrace;  TEOF]. Proof. reflexivity. Qed.
-Lemma lex_wild    : lex "_" = LexOk [TWildcard; TEOF]. Proof. reflexivity. Qed.
-
-Lemma lex_whitespace_ignored :
-  lex "   " = LexOk [TEOF].
-Proof. reflexivity. Qed.
-
-Lemma lex_whitespace_between_tokens :
-  lex "let   x" = LexOk [TLet; TIdent "x"; TEOF].
-Proof. reflexivity. Qed.
-
-Lemma lex_comment_ignored :
-  lex "# this is a comment" = LexOk [TEOF].
-Proof. reflexivity. Qed.
-
-Lemma lex_comment_then_token :
-  lex "# comment
-let" = LexOk [TLet; TEOF].
-Proof. reflexivity. Qed.
-
-Lemma lex_unterminated_string :
-  lex """hello" = LexErr "unterminated string literal".
-Proof. reflexivity. Qed.
-
-Lemma keyword_or_ident_unknown :
-  keyword_or_ident "foobar" = TIdent "foobar".
-Proof. reflexivity. Qed.
-
-Lemma take_while_nil : forall p,
-  take_while p [] = ([], []).
-Proof. intros p. reflexivity. Qed.
-
-Lemma take_while_stops : forall p c cs,
-  p c = false ->
-  take_while p (c :: cs) = ([], c :: cs).
-Proof.
-  intros p c cs H.
-  simpl. rewrite H. reflexivity.
-Qed.
-
-Lemma take_while_matches : forall p c cs,
-  p c = true ->
-  fst (take_while p (c :: cs)) = c :: fst (take_while p cs).
-Proof.
-  intros p c cs H.
-  simpl. rewrite H.
-  destruct (take_while p cs). reflexivity.
-Qed.
