coq/Ast.v
@@ -1,0 +1,174 @@
+From Stdlib Require Import Strings.String.
+From Stdlib Require Import ZArith.ZArith.
+From Stdlib Require Import Lists.List.
+Import ListNotations.
+
+Inductive ty : Type :=
+  | TyInt
+  | TyFloat
+  | TyString
+  | TyBool
+  | TyUnit
+  | TyVar (name : string)
+  | TyList (inner : ty)
+  | TyFun (params : list ty) (ret : ty)
+  | TyAdt (name : string).
+
+Inductive literal : Type :=
+  | LInt (n : Z)
+  | LFloat (s : string)
+  | LString (s : string)
+  | LBool (b : bool)
+  | LUnit
+  | LNil.
+
+Inductive binary_op : Type :=
+  | OpAdd
+  | OpSub
+  | OpMul
+  | OpDiv
+  | OpEqual
+  | OpNotEqual
+  | OpLess
+  | OpGreater
+  | OpCons.
+
+Inductive unary_op : Type :=
+  | OpNegate.
+
+Inductive pattern : Type :=
+  | PWildcard
+  | PVariable (name : string)
+  | PIntLit (n : Z)
+  | PFloatLit (s : string)
+  | PStringLit (s : string)
+  | PBoolLit (b : bool)
+  | PNil
+  | PCons (head : pattern) (tail : pattern)
+  | PConstructor (name : string) (args : list pattern).
+
+Record param : Type := mkParam {
+  param_name : string;
+  param_ty   : option ty;
+}.
+
+Inductive expr : Type :=
+  | Lit (l : literal)
+  | Var (name : string)
+  | Lam (params : list param) (ret_ty : option ty) (body : expr) (is_recursive : bool)
+  | App (f : expr) (args : list expr)
+  | LetE (name : string) (ty : option ty) (body : expr)
+  | IfE (cond : expr) (then_ : expr) (else_ : option expr)
+  | MatchE (scrutinee : expr) (cases : list match_case)
+  | Block (exprs : list expr)
+  | BinOp (op : binary_op) (left : expr) (right : expr)
+  | UnOp (op : unary_op)  (e : expr)
+  | MemberAccess (obj : expr) (field : string)
+  | Range (lo : expr) (hi : expr)
+  | Constructor (name : string) (args : list expr)
+
+with match_case : Type :=
+  | MkCase (pat : pattern) (guard : option expr) (body : expr).
+
+Record import : Type := mkImport {
+  import_module : string;
+  import_item   : string;
+}.
+
+Record variant : Type := mkVariant {
+  variant_name   : string;
+  variant_fields : list ty;
+}.
+
+Record type_decl : Type := mkTypeDecl {
+  type_name : string;
+  variants  : list variant;
+}.
+
+Record program : Type := mkProgram {
+  imports    : list import;
+  type_decls : list type_decl;
+  body       : list expr;
+}.
+
+Definition empty_program : program :=
+  mkProgram [] [] [].
+
+Definition is_empty_program (p : program) : bool :=
+  match p.(body) with
+  | [] => true
+  | _  => false
+  end.
+
+Fixpoint desugar_list (elems : list expr) : expr :=
+  match elems with
+  | [] => Lit LNil
+  | e :: rest => BinOp OpCons e (desugar_list rest)
+  end.
+
+Fixpoint contains_variable (name : string) (e : expr) : bool :=
+  match e with
+  | Lit _ => false
+  | Var nm => String.eqb nm name
+  | Lam _ _ body _ => contains_variable name body
+  | App f args =>
+      orb (contains_variable name f)
+          (existsb (contains_variable name) args)
+  | LetE _ _ body => contains_variable name body
+  | IfE cond then_ else_ =>
+      orb (contains_variable name cond)
+      (orb (contains_variable name then_)
+           (match else_ with
+            | Some e => contains_variable name e
+            | None => false
+            end))
+  | MatchE scrut cases =>
+      orb (contains_variable name scrut)
+          (existsb (fun c =>
+            match c with
+            | MkCase _ guard body =>
+                orb (contains_variable name body)
+                    (match guard with
+                     | Some g => contains_variable name g
+                     | None   => false
+                     end)
+            end) cases)
+  | Block exprs => existsb (contains_variable name) exprs
+  | BinOp _ l r => orb (contains_variable name l) (contains_variable name r)
+  | UnOp _ e => contains_variable name e
+  | MemberAccess obj _ => contains_variable name obj
+  | Range lo hi => orb (contains_variable name lo) (contains_variable name hi)
+  | Constructor _ args => existsb (contains_variable name) args
+  end.
+
+Lemma contains_variable_lit : forall nm l,
+  contains_variable nm (Lit l) = false.
+Proof. intros nm l. reflexivity. Qed.
+
+Lemma contains_variable_var_same : forall nm,
+  contains_variable nm (Var nm) = true.
+Proof. intros nm. simpl. rewrite String.eqb_refl. reflexivity. Qed.
+
+Lemma contains_variable_var_diff : forall nm1 nm2,
+  nm1 <> nm2 -> contains_variable nm1 (Var nm2) = false.
+Proof.
+  intros nm1 nm2 H. simpl.
+  rewrite <- String.eqb_neq in H. rewrite String.eqb_sym. rewrite H. reflexivity.
+Qed.
+
+Lemma desugar_nil : desugar_list [] = Lit LNil.
+Proof. reflexivity. Qed.
+
+Lemma desugar_singleton : forall e,
+  desugar_list [e] = BinOp OpCons e (Lit LNil).
+Proof. intros e. reflexivity. Qed.
+
+Lemma desugar_cons : forall e es,
+  desugar_list (e :: es) = BinOp OpCons e (desugar_list es).
+Proof. intros e es. reflexivity. Qed.
+
+Lemma empty_program_body : (empty_program).(body) = [].
+Proof. reflexivity. Qed.
+
+Lemma is_empty_empty : is_empty_program empty_program = true.
+Proof. reflexivity. Qed.
