coq/Extract.v
@@ -1,5 +1,10 @@
 Require Import Token.
+Require Import Ast.
 Require Import Lexer.
+Require Import Parser.
 Require Import Extraction.
 
-Extraction "lexer.ml" lex lex_result token token_beq token_eq_dec.
+Extraction "lunno.ml"
+  lex lex_result token token_beq
+  parse parse_result program expr ty pattern binary_op unary_op
+  literal match_case param import type_decl variant.
