coq/Lexer_proofs.v
@@ -1,0 +1,431 @@
+From Stdlib Require Import Strings.Ascii.
+From Stdlib Require Import Strings.String.
+From Stdlib Require Import Lists.List.
+From Stdlib Require Import ZArith.
+From Stdlib Require Import Lia.
+
+Import ListNotations.
+Require Import Token.
+Require Import Lexer.
+
+Lemma lex_empty : lex "" = LexOk [TEOF].
+Proof. reflexivity. Qed.
+
+Lemma lex_let : lex "let" = LexOk [TLet; TEOF].
+Proof. reflexivity. Qed.
+
+Lemma lex_if : lex "if" = LexOk [TIf; TEOF]. 
+Proof. reflexivity. Qed.
+
+Lemma lex_then : lex "then" = LexOk [TThen; TEOF]. 
+Proof. reflexivity. Qed.
+
+Lemma lex_else : lex "else" = LexOk [TElse; TEOF]. 
+Proof. reflexivity. Qed.
+
+Lemma lex_match : lex "match" = LexOk [TMatch; TEOF]. 
+Proof. reflexivity. Qed.
+
+Lemma lex_import : lex "import" = LexOk [TImport; TEOF]. 
+Proof. reflexivity. Qed.
+
+Lemma lex_data : lex "data" = LexOk [TData; TEOF]. 
+Proof. reflexivity. Qed.
+
+Lemma lex_true : lex "true" = LexOk [TTrue; TEOF]. 
+Proof. reflexivity. Qed.
+
+Lemma lex_false : lex "false" = LexOk [TFalse; TEOF]. 
+Proof. reflexivity. Qed.
+
+Lemma lex_int_kw : lex "int" = LexOk [TInt; TEOF]. 
+Proof. reflexivity. Qed.
+
+Lemma lex_float_kw : lex "float" = LexOk [TFloat; TEOF]. 
+Proof. reflexivity. Qed.
+
+Lemma lex_string_kw : lex "string" = LexOk [TString; TEOF]. 
+Proof. reflexivity. Qed.
+
+Lemma lex_bool_kw : lex "bool" = LexOk [TBool; TEOF]. 
+Proof. reflexivity. Qed.
+
+Lemma lex_unit_kw : lex "unit" = LexOk [TUnit; TEOF]. 
+Proof. reflexivity. Qed.
+
+Lemma lex_list_kw : lex "list" = LexOk [TList; TEOF]. 
+Proof. reflexivity. Qed.
+
+Lemma lex_arrow : lex "->" = LexOk [TArrow; TEOF]. 
+Proof. reflexivity. Qed.
+
+Lemma lex_lt : lex "<" = LexOk [TLt; TEOF]. 
+Proof. reflexivity. Qed.
+
+Lemma lex_gt : lex ">" = LexOk [TGt; TEOF]. 
+Proof. reflexivity. Qed.
+
+Lemma lex_noteq : lex "<>" = LexOk [TNotEq; TEOF]. 
+Proof. reflexivity. Qed.
+
+Lemma lex_cons : lex "::" = LexOk [TCons; TEOF]. 
+Proof. reflexivity. Qed.
+
+Lemma lex_dotdot : lex ".." = LexOk [TDotDot; TEOF]. 
+Proof. reflexivity. Qed.
+
+Lemma lex_plus : lex "+" = LexOk [TPlus; TEOF]. 
+Proof. reflexivity. Qed.
+
+Lemma lex_minus : lex "-" = LexOk [TMinus; TEOF]. 
+Proof. reflexivity. Qed.
+
+Lemma lex_star : lex "*" = LexOk [TStar; TEOF]. 
+Proof. reflexivity. Qed.
+
+Lemma lex_slash : lex "/" = LexOk [TSlash; TEOF]. 
+Proof. reflexivity. Qed.
+
+Lemma lex_equals : lex "=" = LexOk [TEquals; TEOF]. 
+Proof. reflexivity. Qed.
+
+Lemma lex_pipe : lex "|" = LexOk [TPipe; TEOF]. 
+Proof. reflexivity. Qed.
+
+Lemma lex_colon : lex ":" = LexOk [TColon; TEOF]. 
+Proof. reflexivity. Qed.
+
+Lemma lex_dot : lex "." = LexOk [TDot; TEOF]. 
+Proof. reflexivity. Qed.
+
+Lemma lex_comma : lex "," = LexOk [TComma; TEOF]. 
+Proof. reflexivity. Qed.
+
+Lemma lex_lparen : lex "(" = LexOk [TLParen; TEOF]. 
+Proof. reflexivity. Qed.
+
+Lemma lex_rparen : lex ")" = LexOk [TRParen; TEOF]. 
+Proof. reflexivity. Qed.
+
+Lemma lex_lbrack : lex "[" = LexOk [TLBracket; TEOF]. 
+Proof. reflexivity. Qed.
+
+Lemma lex_rbrack : lex "]" = LexOk [TRBracket; TEOF]. 
+Proof. reflexivity. Qed.
+
+Lemma lex_lbrace : lex "{" = LexOk [TLBrace; TEOF]. 
+Proof. reflexivity. Qed.
+
+Lemma lex_rbrace : lex "}" = LexOk [TRBrace; TEOF]. 
+Proof. reflexivity. Qed.
+
+Lemma lex_wild : lex "_" = LexOk [TWildcard; TEOF]. 
+Proof. reflexivity. Qed.
+
+Lemma lex_intlit_zero : lex "0" = LexOk [TIntLit 0; TEOF].
+Proof. reflexivity. Qed.
+
+Lemma lex_intlit_one : lex "1" = LexOk [TIntLit 1; TEOF].
+Proof. reflexivity. Qed.
+
+Lemma lex_intlit_42 : lex "42" = LexOk [TIntLit 42; TEOF].
+Proof. reflexivity. Qed.
+
+Lemma lex_intlit_large : lex "1000000" = LexOk [TIntLit 1000000; TEOF].
+Proof. reflexivity. Qed.
+
+Lemma lex_intlit_then_dot : lex "1." = LexOk [TIntLit 1; TDot; TEOF].
+Proof. reflexivity. Qed.
+
+Lemma lex_intlit_zero_dot_alpha :
+  lex "0.x" = LexOk [TIntLit 0; TDot; TIdent "x"; TEOF].
+Proof. reflexivity. Qed.
+
+Lemma lex_two_intlits : lex "1 2" = LexOk [TIntLit 1; TIntLit 2; TEOF].
+Proof. reflexivity. Qed.
+
+Lemma lex_int_arith : lex "1 + 2" = LexOk [TIntLit 1; TPlus; TIntLit 2; TEOF].
+Proof. reflexivity. Qed.
+
+Lemma lex_float_basic : lex "3.14" = LexOk [TFloatLit "3.14"; TEOF].
+Proof. reflexivity. Qed.
+
+Lemma lex_float_zero : lex "0.0" = LexOk [TFloatLit "0.0"; TEOF].
+Proof. reflexivity. Qed.
+
+Lemma lex_float_point_five : lex "0.5" = LexOk [TFloatLit "0.5"; TEOF].
+Proof. reflexivity. Qed.
+
+Lemma lex_float_long : lex "3.141592" = LexOk [TFloatLit "3.141592"; TEOF].
+Proof. reflexivity. Qed.
+
+Lemma lex_float_then_plus : lex "1.5 + 2.0" =
+  LexOk [TFloatLit "1.5"; TPlus; TFloatLit "2.0"; TEOF].
+Proof. reflexivity. Qed.
+
+Lemma lex_string_empty :
+  lex (String """"%char (String """"%char EmptyString)) = LexOk [TStringLit ""; TEOF].
+Proof. reflexivity. Qed.
+
+Lemma lex_string_hello :
+  lex (String """"%char "hello" ++ (String """"%char EmptyString))
+  = LexOk [TStringLit "hello"; TEOF].
+Proof. reflexivity. Qed.
+
+Lemma lex_string_with_spaces :
+  lex (String """"%char "hi there" ++ (String """"%char EmptyString))
+  = LexOk [TStringLit "hi there"; TEOF].
+Proof. reflexivity. Qed.
+
+Lemma lex_string_escape_quote :
+  lex (String """"%char (String "a"%char (String "\"%char (String """"%char
+    (String "b"%char (String """"%char EmptyString))))))
+  = LexOk [TStringLit (String "a"%char (String """"%char (String "b"%char EmptyString))); TEOF].
+Proof. reflexivity. Qed.
+
+Lemma lex_string_escape_backslash :
+  lex (String """"%char (String "a"%char (String "\"%char (String "\"%char
+    (String "b"%char (String """"%char EmptyString))))))
+  = LexOk [TStringLit (String "a"%char (String "\"%char (String "b"%char EmptyString))); TEOF].
+Proof. reflexivity. Qed.
+
+Lemma lex_unterminated_string :
+  lex (String """"%char "hello") = LexErr "unterminated string literal".
+Proof. reflexivity. Qed.
+
+Lemma lex_ident_simple : lex "foo" = LexOk [TIdent "foo"; TEOF].
+Proof. reflexivity. Qed.
+
+Lemma lex_ident_single_char : lex "x" = LexOk [TIdent "x"; TEOF].
+Proof. reflexivity. Qed.
+
+Lemma lex_ident_with_digit : lex "foo2" = LexOk [TIdent "foo2"; TEOF].
+Proof. reflexivity. Qed.
+
+Lemma lex_ident_with_underscore : lex "foo_bar" = LexOk [TIdent "foo_bar"; TEOF].
+Proof. reflexivity. Qed.
+
+Lemma lex_ident_underscore_prefix : lex "_foo" = LexOk [TIdent "_foo"; TEOF].
+Proof. reflexivity. Qed.
+
+Lemma lex_ident_double_underscore : lex "__" = LexOk [TIdent "__"; TEOF].
+Proof. reflexivity. Qed.
+
+Lemma lex_ident_caps : lex "MyType" = LexOk [TIdent "MyType"; TEOF].
+Proof. reflexivity. Qed.
+
+Lemma lex_letx_is_ident : lex "letx" = LexOk [TIdent "letx"; TEOF].
+Proof. reflexivity. Qed.
+
+Lemma lex_lets_is_ident : lex "lets" = LexOk [TIdent "lets"; TEOF].
+Proof. reflexivity. Qed.
+
+Lemma lex_let2_is_ident : lex "let2" = LexOk [TIdent "let2"; TEOF].
+Proof. reflexivity. Qed.
+
+Lemma lex_let_underscore_is_ident : lex "let_" = LexOk [TIdent "let_"; TEOF].
+Proof. reflexivity. Qed.
+
+Lemma lex_truefalse_is_ident : lex "truefalse" = LexOk [TIdent "truefalse"; TEOF].
+Proof. reflexivity. Qed.
+
+Lemma lex_iffy_is_ident : lex "iffy" = LexOk [TIdent "iffy"; TEOF].
+Proof. reflexivity. Qed.
+
+Lemma lex_wildcard_in_match : lex "| _" = LexOk [TPipe; TWildcard; TEOF].
+Proof. reflexivity. Qed.
+
+Lemma lex_lt_gt_spaced : lex "< >" = LexOk [TLt; TGt; TEOF].
+Proof. reflexivity. Qed.
+
+Lemma lex_colon_not_cons : lex ": :" = LexOk [TColon; TColon; TEOF].
+Proof. reflexivity. Qed.
+
+Lemma lex_dot_not_dotdot : lex ". ." = LexOk [TDot; TDot; TEOF].
+Proof. reflexivity. Qed.
+
+Lemma lex_minus_then_ident : lex "-x" = LexOk [TMinus; TIdent "x"; TEOF].
+Proof. reflexivity. Qed.
+
+Lemma lex_minus_then_int : lex "-1" = LexOk [TMinus; TIntLit 1; TEOF].
+Proof. reflexivity. Qed.
+
+Lemma lex_cr_ignored :
+  lex (String "013"%char EmptyString) = LexOk [TEOF].
+Proof. reflexivity. Qed.
+
+Lemma lex_ws_between_tokens : lex "let	x" = LexOk [TLet; TIdent "x"; TEOF].
+Proof. reflexivity. Qed.
+
+Lemma lex_empty_comment : lex "#
+let" = LexOk [TLet; TEOF].
+Proof. reflexivity. Qed.
+
+Lemma lex_two_comments : lex "# a
+# b
+let" = LexOk [TLet; TEOF].
+Proof. reflexivity. Qed.
+
+Lemma lex_token_then_comment : lex "let # hi" = LexOk [TLet; TEOF].
+Proof. reflexivity. Qed.
+
+Lemma lex_comment_mid_code :
+  lex "let # hi
+x = 1" = LexOk [TLet; TIdent "x"; TEquals; TIntLit 1; TEOF].
+Proof. reflexivity. Qed.
+
+Lemma koi_let : keyword_or_ident "let" = TLet.    
+Proof. reflexivity. Qed.
+
+Lemma koi_if : keyword_or_ident "if" = TIf.     
+Proof. reflexivity. Qed.
+
+Lemma koi_then : keyword_or_ident "then" = TThen.   
+Proof. reflexivity. Qed.
+
+Lemma koi_else : keyword_or_ident "else" = TElse.   
+Proof. reflexivity. Qed.
+
+Lemma koi_match : keyword_or_ident "match" = TMatch.  
+Proof. reflexivity. Qed.
+
+Lemma koi_import : keyword_or_ident "import" = TImport. 
+Proof. reflexivity. Qed.
+
+Lemma koi_data : keyword_or_ident "data" = TData.   
+Proof. reflexivity. Qed.
+
+Lemma koi_true : keyword_or_ident "true" = TTrue.   
+Proof. reflexivity. Qed.
+
+Lemma koi_false : keyword_or_ident "false" = TFalse.  
+Proof. reflexivity. Qed.
+
+Lemma koi_int : keyword_or_ident "int" = TInt.    
+Proof. reflexivity. Qed.
+
+Lemma koi_float : keyword_or_ident "float" = TFloat.  
+Proof. reflexivity. Qed.
+
+Lemma koi_string : keyword_or_ident "string" = TString. 
+Proof. reflexivity. Qed.
+
+Lemma koi_bool : keyword_or_ident "bool" = TBool.   
+Proof. reflexivity. Qed.
+
+Lemma koi_unit : keyword_or_ident "unit" = TUnit.   
+Proof. reflexivity. Qed.
+
+Lemma koi_list : keyword_or_ident "list" = TList.   
+Proof. reflexivity. Qed.
+
+Lemma koi_ident : keyword_or_ident "foobar" = TIdent "foobar". 
+Proof. reflexivity. Qed.
+
+Lemma koi_empty : keyword_or_ident "" = TIdent "". 
+Proof. reflexivity. Qed.
+
+Lemma parse_int_empty : parse_int [] 0%Z = 0%Z.
+Proof. reflexivity. Qed.
+
+Lemma parse_int_zero : parse_int ["0"%char] 0%Z = 0%Z.
+Proof. reflexivity. Qed.
+
+Lemma parse_int_one : parse_int ["1"%char] 0%Z = 1%Z.
+Proof. reflexivity. Qed.
+
+Lemma parse_int_42 : parse_int ["4"%char; "2"%char] 0%Z = 42%Z.
+Proof. reflexivity. Qed.
+
+Lemma parse_int_acc : parse_int ["5"%char] 10%Z = 105%Z.
+Proof. reflexivity. Qed.
+
+Lemma take_while_all_match : forall (cs : list ascii),
+  (forall c, In c cs -> is_digit c = true) ->
+  snd (take_while is_digit cs) = [].
+Proof.
+  induction cs as [| c rest IH].
+  - intros _. reflexivity.
+  - intros H.
+    simpl. rewrite (H c (or_introl eq_refl)).
+    destruct (take_while is_digit rest) as [taken remaining] eqn:E.
+    simpl. apply IH.
+    intros x Hx. apply H. right. exact Hx.
+Qed.
+
+Lemma take_while_append : forall p cs taken remaining,
+  take_while p cs = (taken, remaining) ->
+  cs = taken ++ remaining.
+Proof.
+  intros p cs. induction cs as [| c rest IH];
+  intros taken remaining H.
+  - simpl in H. injection H as <- <-. reflexivity.
+  - simpl in H. destruct (p c) eqn:Hpc.
+    + destruct (take_while p rest) as [t r] eqn:E.
+      injection H as <- <-. simpl. f_equal.
+      apply (IH t r). reflexivity.
+    + injection H as <- <-. reflexivity.
+Qed.
+
+Lemma take_while_length : forall p cs taken remaining,
+  take_while p cs = (taken, remaining) ->
+  length taken + length remaining = length cs.
+Proof.
+  intros p cs taken remaining H.
+  apply take_while_append in H.
+  rewrite H. rewrite length_app. lia.
+Qed.
+
+Lemma lex_let_binding :
+  lex "let x = 42" = LexOk [TLet; TIdent "x"; TEquals; TIntLit 42; TEOF].
+Proof. reflexivity. Qed.
+
+Lemma lex_if_expr :
+  lex "if true then 1 else 0" =
+  LexOk [TIf; TTrue; TThen; TIntLit 1; TElse; TIntLit 0; TEOF].
+Proof. reflexivity. Qed.
+
+Lemma lex_cons_list :
+  lex "1 :: 2 :: []" =
+  LexOk [TIntLit 1; TCons; TIntLit 2; TCons; TLBracket; TRBracket; TEOF].
+Proof. reflexivity. Qed.
+
+Lemma lex_match_expr :
+  lex "match x | _ -> 1" =
+  LexOk [TMatch; TIdent "x"; TPipe; TWildcard; TArrow; TIntLit 1; TEOF].
+Proof. reflexivity. Qed.
+
+Lemma lex_type_annotation :
+  lex "x : int" = LexOk [TIdent "x"; TColon; TInt; TEOF].
+Proof. reflexivity. Qed.
+
+Lemma lex_fn_type :
+  lex "int -> bool" = LexOk [TInt; TArrow; TBool; TEOF].
+Proof. reflexivity. Qed.
+
+Lemma lex_list_literal :
+  lex "[1, 2, 3]" =
+  LexOk [TLBracket; TIntLit 1; TComma; TIntLit 2; TComma; TIntLit 3;
+         TRBracket; TEOF].
+Proof. reflexivity. Qed.
+
+Lemma lex_member_access :
+  lex "foo.bar" = LexOk [TIdent "foo"; TDot; TIdent "bar"; TEOF].
+Proof. reflexivity. Qed.
+
+Lemma lex_range :
+  lex "[0..10]" =
+  LexOk [TLBracket; TIntLit 0; TDotDot; TIntLit 10; TRBracket; TEOF].
+Proof. reflexivity. Qed.
+
+Lemma lex_not_equal :
+  lex "x <> y" = LexOk [TIdent "x"; TNotEq; TIdent "y"; TEOF].
+Proof. reflexivity. Qed.
+
+Lemma lex_comparison :
+  lex "x < y" = LexOk [TIdent "x"; TLt; TIdent "y"; TEOF].
+Proof. reflexivity. Qed.
+
+Lemma lex_import_expr :
+  lex "import ""core:io""" = LexOk [TImport; TStringLit "core:io"; TEOF].
+Proof. reflexivity. Qed.
