coq/Parser_proofs.v
@@ -1,0 +1,22 @@
+From Stdlib Require Import Strings.Ascii.
+From Stdlib Require Import Strings.String.
+From Stdlib Require Import Lists.List.
+From Stdlib Require Import ZArith.
+From Stdlib Require Import Lia.
+
+Import ListNotations.
+Require Import Token.
+Require Import Ast.
+Require Import Lexer.
+Require Import Parser.
+
+Lemma parse_empty : parse [TEOF] = ParseOk empty_program [TEOF].
+Proof. vm_compute. reflexivity. Qed.
+
+Lemma parse_int_lit :
+  parse [TIntLit 42; TEOF] = ParseOk (mkProgram [] [] [Lit (LInt 42)]) [TEOF].
+Proof. vm_compute. reflexivity. Qed.
+
+Lemma parse_true :
+  parse [TTrue; TEOF] = ParseOk (mkProgram [] [] [Lit (LBool true)]) [TEOF].
+Proof. vm_compute. reflexivity. Qed.
